src/Assembly/WordizeUtil.v
@@ -1,6 +1,6 @@
 Require Import Bedrock.Word Bedrock.Nomega.
 Require Import NArith PArith Ndigits Nnat NPow NPeano Ndec.
-Require Import List Omega NArith Nnat BoolEq.
+Require Import List Omega NArith Nnat BoolEq Compare_dec.
 Require Import SetoidTactics.
 Require Import ProofIrrelevance FunctionalExtensionality.
 Require Import QhasmUtil QhasmEvalCommon.
@@ -22,12 +22,12 @@ Section Misc.
 
     - unfold N.lt; rewrite N2Nat.inj_compare.
       repeat rewrite Nat2N.id.
-      apply Nat.compare_lt_iff in H.
+      apply nat_compare_lt in H.
       intuition.
 
     - unfold N.lt in H; rewrite N2Nat.inj_compare in H.
       repeat rewrite Nat2N.id in H.
-      apply Nat.compare_lt_iff in H.
+      apply nat_compare_lt in H.
       intuition.
   Qed.
 
@@ -36,11 +36,11 @@ Section Misc.
     intros x b; split; intro H.
 
     - unfold N.lt in H; rewrite N2Nat.inj_compare in H.
-      apply Nat.compare_lt_iff in H.
+      apply nat_compare_lt in H.
       intuition.
 
     - unfold N.lt; rewrite N2Nat.inj_compare.
-      apply Nat.compare_lt_iff.
+      apply nat_compare_lt.
       intuition.
   Qed.
 
@@ -189,7 +189,7 @@ Section Exp.
     unfold N.lt.
     rewrite N2Nat.inj_compare.
     rewrite Nat2N.id.
-    apply Nat.compare_lt_iff in H.
+    apply nat_compare_lt in H.
     assumption.
   Qed.
 
@@ -317,351 +317,26 @@ Section Conversions.
   Qed.
 End Conversions.
 
-Section Enumerability.
-  Class Enumerable A := {
-    elements : list A;
-    correct : forall x: A, In x elements;
-    good: NoDup elements;
-    }.
-
-  Arguments elements _ {_}.
-
-  Definition word_elements (n: nat): list (word n) :=
-    map (natToWord n) (seq O (pow2 n)).
-
-  Lemma word_index_correct : forall n (x: word n),
-    x = nth (wordToNat x) (word_elements n) (natToWord _ 0).
-  Proof.
-    intros; unfold word_elements.
-    rewrite map_nth.
-    rewrite seq_nth; try apply wordToNat_bound; simpl.
-    rewrite natToWord_wordToNat.
-    reflexivity.
-  Qed.
-
-  Lemma word_elements_correct: forall n (x: word n),
-      In x (word_elements n).
-  Proof.
-    intros; unfold word_elements.
-    destruct (nth_in_or_default (wordToNat x) (word_elements n) (natToWord _ 0)).
-
-    - rewrite <- word_index_correct in i.
-        assumption.
-
-    - rewrite <- word_index_correct in e.
-        apply in_map_iff.
-        exists 0; split; simpl; intuition.
-        apply in_seq.
-        pose proof (pow2_gt0 n).
-        omega.
-  Qed.
-
-  Lemma word_elements_good: forall n, NoDup (word_elements n).
-  Proof.
-    intros; unfold word_elements.
-
-    apply <- (NoDup_nth (map (natToWord n) (seq 0 (pow2 n))) (natToWord _ 0)).
-
-    intros; repeat rewrite map_nth in H1.
-
-    rewrite map_length in H, H0.
-    rewrite seq_length in H, H0.
-
-    replace (nth i (seq 0 (pow2 n)) 0) with i in H1
-        by (rewrite seq_nth; simpl; intuition).
-    replace (nth j (seq 0 (pow2 n)) 0) with j in H1
-        by (rewrite seq_nth; simpl; intuition).
-
-    rewrite <- (@wordToNat_natToWord_idempotent n i);
-        try apply pow2_N_bound; intuition
-    rewrite <- (@wordToNat_natToWord_idempotent n j);
-        try apply pow2_N_bound; intuition
-    rewrite H1; intuition.
-
-  Qed.
-
-  Instance word_enumerable: forall n, Enumerable (word n) := {
-    elements := word_elements n;
-    correct := word_elements_correct n;
-    good := word_elements_good n
-  }.
-
-  Lemma word_enum_correct: forall n e, length (@elements (word n) e) = pow2 n.
-  Proof.
-    intros.
-    destruct e as [nelem ncorrect ngood].
-    induction n.
-
-    - simpl; inversion ngood.
-
-      + rewrite <- H in ncorrect.
-        pose proof (ncorrect WO).
-        inversion H0.
-
-      + rewrite (shatter_word_0 x) in *.
-        destruct (list_eq_dec (@weq 0) l nil); subst; intuition.
-        contradict H.
-        induction l.
-
-        * apply n; intuition.
-
-        * rewrite (shatter_word_0 a).
-          intuition.
-
-    - replace (pow2 (S n)) with (2 * pow2 n) by (simpl; intuition).
-      unfold elements; cbv zeta.
-
-      assert (exists l1 l2, partition (@whd _) nelem = (l1, l2)) as H by (
-        destruct (partition (@whd _) nelem) as [l l0];
-                  exists l; exists l0; intuition).
-
-      destruct H as [l1 H].
-      destruct H as [l2 H].
-
-      assert (forall x : word n, In x (map (split2 1 n) l1))
-          as ncorrect1. {
-        intro. clear ngood IHn.
-
-        replace x with (split2 1 n (WS true x)) by (simpl; intuition).
-        apply in_map.
-
-        pose proof (ncorrect (WS true x)) as ncorrect'; clear ncorrect.
-
-        revert ncorrect'; revert x H; revert l1 l2; induction nelem; intros.
-
-        - inversion ncorrect'.
-
-        - destruct ncorrect'; subst.
-
-          + simpl in H.
-            destruct (partition (whd (sz:=n)) nelem) as [g d].
-            inversion H.
-            intuition.
-
-          + simpl in H; destruct (whd a); simpl in H;
-              destruct (partition (whd (sz:=n)) nelem) as [g d];
-              inversion H; subst; clear H.
-
-            * right; apply (IHnelem g l2); intuition.
-
-            * apply (IHnelem l1 d); intuition.
-      }
-
-      assert (forall x : word n, In x (map (split2 1 n) l2))
-          as ncorrect2. {
-        intro. clear ngood IHn ncorrect1.
-
-        replace x with (split2 1 n (WS false x)) by (simpl; intuition).
-        apply in_map.
-
-        pose proof (ncorrect (WS false x)) as ncorrect'; clear ncorrect.
-
-        revert ncorrect'; revert x H; revert l1 l2; induction nelem; intros.
-
-        - inversion ncorrect'.
-
-        - destruct ncorrect'; subst.
-
-          + simpl in H.
-            destruct (partition (whd (sz:=n)) nelem) as [g d].
-            inversion H.
-            intuition.
-
-          + simpl in H; destruct (whd a); simpl in H;
-              destruct (partition (whd (sz:=n)) nelem) as [g d];
-              inversion H; subst; clear H.
-
-            * apply (IHnelem g); intuition.
-
-            * right; apply (IHnelem l1); intuition.
-      }
-
-      assert (NoDup (map (split2 1 n) l1)) as ngood1. {
-        clear ncorrect1 ncorrect2 IHn ncorrect.
-        revert ngood H; revert l1 l2; induction nelem; intros.
-
-        - simpl in H; inversion H; subst; clear H.
-            simpl; constructor.
-
-        - inversion ngood; subst; clear ngood.
-
-          assert (exists g d, partition (@whd n) nelem = (g, d)) as E by (
-                destruct (partition _ _) as [g d]; exists g; exists d; intuition);
-          destruct E as [g E]; destruct E as [d E].
-
-          pose proof (elements_in_partition _ _ E) as I.
-
-          destruct (shatter_word_S a) as [b Q].
-          destruct Q as [a' Ha].
-          rewrite Ha in *; simpl in H.
-
-          simpl in H; destruct b; rewrite E in *;
-            inversion H; subst; clear H.
-
-          + constructor. 
-
-            * intro H; clear IHnelem.
-
-              pose proof (@in_map_iff (word (S n)) (word n) (@wtl n) g a') as M.
-              apply M in H; clear M; destruct H; destruct H as [Ha Hb].
-              assert (whd x = true) as Hhd. {
-                clear I H2 H3 Ha a'.
-                destruct (shatter_word_S x) as [b H];
-                  destruct H as [x' H]; rewrite H in *; clear H x; simpl.
-
-                revert Hb E. revert x' b g l2.
-                induction nelem; intros; simpl in E.
-
-                - inversion E; subst.
-                    inversion Hb.
-
-                - simpl in E;
-                    destruct (bool_dec (whd a) true) as [B|B];
-                    destruct (partition (whd (sz:=n)) nelem) as [g' d'].
-
-                  + rewrite B in E; inversion E; subst; clear E;
-                      destruct Hb.
-
-                    * rewrite H in *; simpl in B; intuition.
-
-                    * apply (IHnelem x' b g' l2); intuition.
-
-                  + assert (whd a = false) as B' by (
-                      induction (whd a); intuition); clear B.
-
-                    rewrite B' in E. inversion E. subst. clear E.
-                    apply (IHnelem x' b g d'); intuition.
-              }
-
-              destruct (shatter_word_S x) as [b H].
-              destruct H as [x' H].
-              rewrite H in *; simpl in *; clear H.
-              rewrite Hhd in Hb.
-              rewrite Ha in Hb.
-              assert (In (a'~1) g \/ In (a'~1) l2) as Q by intuition.
-              apply I in Q.
-              intuition.
-
-            * apply (IHnelem g l2); intuition.
-
-            + apply (IHnelem _ d); intuition.
-      }
-
-      assert (NoDup (map (split2 1 n) l2)) as ngood2. {
-        clear ncorrect1 ncorrect2 IHn ncorrect ngood1.
-        revert ngood H; revert l1 l2; induction nelem; intros.
-
-        - simpl in H; inversion H; subst; clear H.
-          simpl; constructor.
-
-        - inversion ngood; subst; clear ngood.
-
-          assert (exists g d, partition (@whd n) nelem = (g, d)) as E by (
-              destruct (partition _ _) as [g d]; exists g; exists d; intuition);
-            destruct E as [g E];
-            destruct E as [d E].
-
-          pose proof (elements_in_partition _ _ E) as I.
-
-          destruct (shatter_word_S a) as [b Q].
-          destruct Q as [a' Ha].
-          rewrite Ha in *; simpl in H.
-
-          simpl in H; destruct b; rewrite E in *;
-          inversion H; subst; clear H.
-
-          + apply (IHnelem g l2); intuition.
-
-          + constructor. 
-
-            * intro H; clear IHnelem.
-
-              pose proof (@in_map_iff (word (S n)) (word n) (@wtl n) d a') as M.
-              apply M in H; clear M; destruct H; destruct H as [Ha Hb].
-              assert (whd x = false) as Hhd. {
-                clear I H2 H3 Ha a'.
-                destruct (shatter_word_S x) as [b H];
-                    destruct H as [x' H]; rewrite H in *; clear H x; simpl.
-
-                revert Hb E. revert x' b d l1.
-                induction nelem; intros; simpl in E.
-
-                - inversion E; subst.
-                    inversion Hb.
-
-                - simpl in E;
-                    destruct (bool_dec (whd a) false) as [B|B];
-                    destruct (partition (whd (sz:=n)) nelem) as [g' d'].
-
-                  + rewrite B in E; inversion E; subst; clear E;
-                      destruct Hb.
-
-                    * rewrite H in *; simpl in B; intuition.
-
-                    * apply (IHnelem x' b d' l1); intuition.
-
-                    + assert (whd a = true) as B' by (
-                        induction (whd a); intuition); clear B.
-                  rewrite B' in E. inversion E. subst. clear E.
-                  apply (IHnelem x' b d g'); intuition.
-              }
-
-              destruct (shatter_word_S x) as [b H].
-              destruct H as [x' H].
-              rewrite H in *; simpl in *; clear H.
-              rewrite Hhd in Hb.
-              rewrite Ha in Hb.
-              assert (In (a'~0) l1 \/ In (a'~0) d) as Q by intuition.
-              apply I in Q.
-              intuition.
-
-            * apply (IHnelem l1 d); intuition.
-      }
-
-      pose proof (IHn _ ncorrect1 ngood1) as H1;
-        unfold elements in H1; rewrite map_length in H1.
-
-      pose proof (IHn _ ncorrect2 ngood2) as H2;
-        unfold elements in H2; rewrite map_length in H2.
-
-      rewrite (partition_length _ _ H); simpl in *.
-      rewrite H1, H2.
-      omega.
-  Qed.
-
-  Lemma word_equiv_correct: forall n m, word n = word m -> n = m.
-  Proof.
-    intros n m H.
-    apply pow2_inv.
-
-    pose proof (word_enum_correct n) as Hn.
-    pose proof (word_enum_correct m) as Hm.
-
-    rewrite H in Hn.
-    rewrite <- (Hn (word_enumerable m)).
-    rewrite <- (Hm (word_enumerable m)).
-
-    reflexivity.
-  Qed.
-End Enumerability.
-
 Section SpecialFunctions.
   Local Open Scope nword_scope.
 
-  Lemma convS_id: forall A x p, (@convS A A x p) = x.
+  Lemma convS_id: forall n x p, (@convS n n x p) = x.
   Proof.
     intros; unfold convS; vm_compute.
-    replace p with (eq_refl A); intuition.
-    apply proof_irrelevance.
+    replace (convS_subproof n n x p)
+      with (eq_refl (word n)) by (apply proof_irrelevance).
+    reflexivity.
   Qed.
 
   Lemma wordToN_convS: forall {n m} x p,
-    wordToN (@convS (word n) (word m) x p) = wordToN x.
+    wordToN (@convS n m x p) = wordToN x.
   Proof.
     intros.
-    pose proof (word_equiv_correct _ _ p) as H.
-    revert x p; rewrite H; intros.
-    rewrite convS_id; reflexivity.
+    revert x.
+    rewrite p.
+    intro x.
+    rewrite convS_id.
+    reflexivity.
   Qed.
 
   Lemma wordToN_zext: forall {n m} (x: word n),
@@ -883,17 +558,17 @@ Section SpecialFunctions.
       replace (& wones (S x)) with (2 * & (wones x) + N.b2n true)%N
         by (simpl; nomega).
       replace (N.ones (N.succ _))
-         with (2 * N.ones (N.of_nat x) + N.b2n true)%N
-           by (
-        replace (N.succ (N.of_nat x)) with (1 + (N.of_nat x))%N by (
-          rewrite N.add_comm; nomega);
-        rewrite N.ones_add;
+         with (2 * N.ones (N.of_nat x) + N.b2n true)%N.
+
+      + rewrite IHx; nomega.
+
+      + replace (N.succ (N.of_nat x)) with (1 + (N.of_nat x))%N by (
+          rewrite N.add_comm; nomega).
+        rewrite N.ones_add.
         replace (N.ones 1) with 1%N by (
-          unfold N.ones; simpl; intuition);
-        simpl; reflexivity).
- 
-      rewrite IHx.
-      nomega.
+          unfold N.ones; simpl; intuition).
+        simpl.
+        reflexivity.
   Qed.
 
   Ltac propagate_wordToN :=
